theories/NormalForms.v
@@ -51,6 +51,7 @@ with dne : term -> Set :=
   | dne_tSnd {n} : dne n -> dne (tSnd n)
   | dne_tIdElim {A x P hr y e} : dnf A -> dnf x -> dnf P -> dnf hr -> dnf y -> dne e -> dne (tIdElim A x P hr y e)
   | dne_tQuote {t} : ~ closed0 t -> dnf t -> dne (tQuote t)
+  | dne_tStep {t u} : (~ is_closedn 0 t) + (~ is_closedn 0 u) -> dnf t -> dnf u -> dne (tStep t u)
   | dne_tReflect {t u} : (~ is_closedn 0 t) + (~ is_closedn 0 u) -> dnf t -> dnf u -> dne (tReflect t u)
 .
 
@@ -60,10 +61,10 @@ Scheme
   Induction for dnf Sort Type with
   Induction for dne Sort Type.
 
-Definition dnf_dne_rect P Q p1 p2 p3 p4 p5 p6 p7 p8 p9 p10 p11 p12 p13 p14 p15 p16 p17 p18 p19 p20 p21 :=
+Definition dnf_dne_rect P Q p1 p2 p3 p4 p5 p6 p7 p8 p9 p10 p11 p12 p13 p14 p15 p16 p17 p18 p19 p20 p21 p22 :=
   pair
-    (dnf_rect P Q p1 p2 p3 p4 p5 p6 p7 p8 p9 p10 p11 p12 p13 p14 p15 p16 p17 p18 p19 p20 p21)
-    (dne_rect P Q p1 p2 p3 p4 p5 p6 p7 p8 p9 p10 p11 p12 p13 p14 p15 p16 p17 p18 p19 p20 p21).
+    (dnf_rect P Q p1 p2 p3 p4 p5 p6 p7 p8 p9 p10 p11 p12 p13 p14 p15 p16 p17 p18 p19 p20 p21 p22)
+    (dne_rect P Q p1 p2 p3 p4 p5 p6 p7 p8 p9 p10 p11 p12 p13 p14 p15 p16 p17 p18 p19 p20 p21 p22).
 
 (** ** Weak-head normal forms and neutrals. *)
 
@@ -89,6 +90,7 @@ with whne : term -> Type :=
   | whne_tSnd {p} : whne p -> whne (tSnd p)
   | whne_tIdElim {A x P hr y e} : whne e -> whne (tIdElim A x P hr y e)
   | whne_tQuote {t} :  ~ closed0 t -> dnf t -> whne (tQuote t)
+  | whne_tStep {t u} : (~ is_closedn 0 t) + (~ is_closedn 0 u) -> dnf t -> dnf u -> whne (tStep t u)
   | whne_tReflect {t u} : (~ is_closedn 0 t) + (~ is_closedn 0 u) -> dnf t -> dnf u -> whne (tReflect t u)
 .
 
@@ -140,7 +142,8 @@ Lemma closed0_whne : forall t, closed0 t -> whne t -> False.
 Proof.
 unfold closed0; intros t Hc Ht; induction Ht; cbn in *; eauto.
 all: repeat match goal with H : _ |- _ => apply andb_prop in H; destruct H end; eauto.
-destruct s; congruence.
++ destruct s; congruence.
++ destruct s; congruence.
 Qed.
 
 Section RenDnf.
@@ -149,6 +152,9 @@ Lemma dnf_dne_ren : (forall t, dnf t -> forall ρ, dnf t⟨ρ⟩) × (forall t, 
 Proof.
 apply dnf_dne_rect; cbn; intros; try now econstructor.
 + constructor; [|now eauto].
+  intros Hc; now apply closed0_ren_rev in Hc.
++ constructor; [|now eauto|now eauto].
+  destruct s; [left|right];
   intros Hc; now apply closed0_ren_rev in Hc.
 + constructor; [|now eauto|now eauto].
   destruct s; [left|right];
@@ -176,6 +182,12 @@ all: try now (
   do 2 constructor; [now eintros ?%closed0_ren|eauto].
 + inversion H; subst.
   constructor; [now eintros ?%closed0_ren|eauto].
++ inversion H; subst; inversion H4; subst.
+  do 2 constructor; eauto.
+  destruct H7; [left|right]; now eintros ?%closed0_ren.
++ inversion H; subst.
+  constructor; eauto.
+  destruct H6; [left|right]; now eintros ?%closed0_ren.
 + inversion H; subst; inversion H4; subst.
   do 2 constructor; eauto.
   destruct H7; [left|right]; now eintros ?%closed0_ren.
@@ -312,6 +324,8 @@ Section RenWhnf.
       intros Hc; now apply closed0_ren_rev in Hc.
     + econstructor; try now eapply dnf_ren.
       destruct s; [left|right]; intros Hc; now apply closed0_ren_rev in Hc.
+    + econstructor; try now eapply dnf_ren.
+      destruct s; [left|right]; intros Hc; now apply closed0_ren_rev in Hc.
   Qed.
 
   Lemma whnf_ren t : whnf t -> whnf (t⟨ρ⟩).
@@ -380,6 +394,7 @@ Fixpoint is_nf ne t {struct t} := match t with
 | tIdElim A x P hr y e =>
   is_nf false A && is_nf false x && is_nf false P && is_nf false hr && is_nf false y && is_nf true e
 | tQuote t => is_nf false t && negb (is_closedn 0 t)
+| tStep t u => is_nf false t && is_nf false u && (negb (is_closedn 0 t) || negb (is_closedn 0 u))
 | tReflect t u => is_nf false t && is_nf false u && (negb (is_closedn 0 t) || negb (is_closedn 0 u))
 end.
 
@@ -403,6 +418,7 @@ Fixpoint is_wnf ne t {struct t} := match t with
 | tSnd t => is_wnf true t
 | tIdElim A x P hr y e => is_wnf true e
 | tQuote t => is_dnf t && negb (is_closedn 0 t)
+| tStep t u => is_dnf t && is_dnf u && (negb (is_closedn 0 t) || negb (is_closedn 0 u))
 | tReflect t u => is_dnf t && is_dnf u && (negb (is_closedn 0 t) || negb (is_closedn 0 u))
 end.
 
@@ -424,6 +440,7 @@ all: repeat (apply andb_true_intro; split); eauto.
 + now apply is_nf_incl.
 + now apply Bool.eq_true_not_negb.
 + apply Bool.orb_true_intro; destruct s; [left|right]; now apply Bool.eq_true_not_negb.
++ apply Bool.orb_true_intro; destruct s; [left|right]; now apply Bool.eq_true_not_negb.
 Qed.
 
 Lemma is_nf_dnf_dne :
@@ -438,6 +455,8 @@ all: try match goal with |- dne _ => constructor end.
 all: eauto using dnf, dne.
 + now eapply contraNnot.
 + now eapply contraNnot.
++ apply Bool.orb_true_elim in H0; destruct H0; [left|right]; now eapply contraNnot.
++ apply Bool.orb_true_elim in H0; destruct H0; [left|right]; now eapply contraNnot.
 + apply Bool.orb_true_elim in H0; destruct H0; [left|right]; now eapply contraNnot.
 + apply Bool.orb_true_elim in H0; destruct H0; [left|right]; now eapply contraNnot.
 Qed.
@@ -471,6 +490,9 @@ all: repeat (apply andb_true_intro; split); eauto using whne, whnf.
 + now eapply dnf_dne_is_nf.
 + now eapply dnf_dne_is_nf.
 + apply Bool.orb_true_intro; destruct s; [left|right]; now apply Bool.eq_true_not_negb.
++ now eapply dnf_dne_is_nf.
++ now eapply dnf_dne_is_nf.
++ apply Bool.orb_true_intro; destruct s; [left|right]; now apply Bool.eq_true_not_negb.
 Qed.
 
 Lemma is_whne_whne : forall t, is_whne t = true -> whne t.
@@ -481,6 +503,8 @@ all: eauto using whne, whnf.
 + constructor.
   - unfold closed0; destruct is_closedn; cbn in *; congruence.
   - now apply is_nf_dnf_dne.
++ constructor; try now apply is_nf_dnf_dne.
+  apply Bool.orb_true_elim in H0; destruct H0; [left|right]; now eapply contraNnot.
 + constructor; try now apply is_nf_dnf_dne.
   apply Bool.orb_true_elim in H0; destruct H0; [left|right]; now eapply contraNnot.
 Qed.
